with Megan, fixing some error messages, workarounds in records, but a main step in L0.Core goes through (very verbose)

pulse/src/ocaml/plugin/generated/Pulse_Checker_Rewrite.ml
@@ -23,7 +23,7 @@ let (check_rewrite :
                  (Obj.magic
                     (FStar_Range.mk_range "Pulse.Checker.Rewrite.fst"
                        (Prims.of_int (20)) (Prims.of_int (51))
-                       (Prims.of_int (33)) (Prims.of_int (72)))))
+                       (Prims.of_int (42)) (Prims.of_int (72)))))
               (FStar_Tactics_Effect.lift_div_tac
                  (fun uu___ ->
                     Pulse_Checker_Pure.push_context "check_rewrite"
@@ -43,7 +43,7 @@ let (check_rewrite :
                                (FStar_Range.mk_range
                                   "Pulse.Checker.Rewrite.fst"
                                   (Prims.of_int (20)) (Prims.of_int (51))
-                                  (Prims.of_int (33)) (Prims.of_int (72)))))
+                                  (Prims.of_int (42)) (Prims.of_int (72)))))
                          (FStar_Tactics_Effect.lift_div_tac
                             (fun uu___ -> t.Pulse_Syntax_Base.term1))
                          (fun uu___ ->
@@ -69,7 +69,7 @@ let (check_rewrite :
                                                  "Pulse.Checker.Rewrite.fst"
                                                  (Prims.of_int (21))
                                                  (Prims.of_int (41))
-                                                 (Prims.of_int (33))
+                                                 (Prims.of_int (42))
                                                  (Prims.of_int (72)))))
                                         (Obj.magic
                                            (Pulse_Checker_Pure.check_vprop g1
@@ -95,7 +95,7 @@ let (check_rewrite :
                                                                 "Pulse.Checker.Rewrite.fst"
                                                                 (Prims.of_int (22))
                                                                 (Prims.of_int (44))
-                                                                (Prims.of_int (33))
+                                                                (Prims.of_int (42))
                                                                 (Prims.of_int (72)))))
                                                        (Obj.magic
                                                           (Pulse_Checker_Pure.check_vprop
@@ -116,15 +116,15 @@ let (check_rewrite :
                                                                     "Pulse.Checker.Rewrite.fst"
                                                                     (Prims.of_int (25))
                                                                     (Prims.of_int (6))
-                                                                    (Prims.of_int (31))
-                                                                    (Prims.of_int (48)))))
+                                                                    (Prims.of_int (40))
+                                                                    (Prims.of_int (30)))))
                                                                     (FStar_Sealed.seal
                                                                     (Obj.magic
                                                                     (FStar_Range.mk_range
                                                                     "Pulse.Checker.Rewrite.fst"
-                                                                    (Prims.of_int (31))
-                                                                    (Prims.of_int (51))
+                                                                    (Prims.of_int (40))
                                                                     (Prims.of_int (33))
+                                                                    (Prims.of_int (42))
                                                                     (Prims.of_int (72)))))
                                                                     (if
                                                                     Pulse_Syntax_Base.eq_tm
@@ -145,25 +145,77 @@ let (check_rewrite :
                                                                     (FStar_Range.mk_range
                                                                     "Pulse.Checker.Rewrite.fst"
                                                                     (Prims.of_int (27))
-                                                                    (Prims.of_int (17))
+                                                                    (Prims.of_int (24))
                                                                     (Prims.of_int (27))
-                                                                    (Prims.of_int (71)))))
+                                                                    (Prims.of_int (35)))))
                                                                     (FStar_Sealed.seal
                                                                     (Obj.magic
                                                                     (FStar_Range.mk_range
                                                                     "Pulse.Checker.Rewrite.fst"
                                                                     (Prims.of_int (27))
-                                                                    (Prims.of_int (11))
-                                                                    (Prims.of_int (31))
-                                                                    (Prims.of_int (48)))))
+                                                                    (Prims.of_int (38))
+                                                                    (Prims.of_int (40))
+                                                                    (Prims.of_int (30)))))
+                                                                    (FStar_Tactics_Effect.lift_div_tac
+                                                                    (fun
+                                                                    uu___4 ->
+                                                                    Pulse_Elaborate_Pure.elab_term
+                                                                    p1))
+                                                                    (fun
+                                                                    uu___4 ->
+                                                                    (fun
+                                                                    elab_p ->
+                                                                    Obj.magic
+                                                                    (FStar_Tactics_Effect.tac_bind
+                                                                    (FStar_Sealed.seal
+                                                                    (Obj.magic
+                                                                    (FStar_Range.mk_range
+                                                                    "Pulse.Checker.Rewrite.fst"
+                                                                    (Prims.of_int (28))
+                                                                    (Prims.of_int (24))
+                                                                    (Prims.of_int (28))
+                                                                    (Prims.of_int (35)))))
+                                                                    (FStar_Sealed.seal
+                                                                    (Obj.magic
+                                                                    (FStar_Range.mk_range
+                                                                    "Pulse.Checker.Rewrite.fst"
+                                                                    (Prims.of_int (28))
+                                                                    (Prims.of_int (38))
+                                                                    (Prims.of_int (40))
+                                                                    (Prims.of_int (30)))))
+                                                                    (FStar_Tactics_Effect.lift_div_tac
+                                                                    (fun
+                                                                    uu___4 ->
+                                                                    Pulse_Elaborate_Pure.elab_term
+                                                                    q1))
+                                                                    (fun
+                                                                    uu___4 ->
+                                                                    (fun
+                                                                    elab_q ->
+                                                                    Obj.magic
+                                                                    (FStar_Tactics_Effect.tac_bind
+                                                                    (FStar_Sealed.seal
+                                                                    (Obj.magic
+                                                                    (FStar_Range.mk_range
+                                                                    "Pulse.Checker.Rewrite.fst"
+                                                                    (Prims.of_int (29))
+                                                                    (Prims.of_int (29))
+                                                                    (Prims.of_int (29))
+                                                                    (Prims.of_int (69)))))
+                                                                    (FStar_Sealed.seal
+                                                                    (Obj.magic
+                                                                    (FStar_Range.mk_range
+                                                                    "Pulse.Checker.Rewrite.fst"
+                                                                    (Prims.of_int (28))
+                                                                    (Prims.of_int (38))
+                                                                    (Prims.of_int (40))
+                                                                    (Prims.of_int (30)))))
                                                                     (Obj.magic
                                                                     (FStar_Tactics_V2_Builtins.check_equiv
                                                                     (Pulse_Typing.elab_env
                                                                     g1)
-                                                                    (Pulse_Elaborate_Pure.elab_term
-                                                                    p1)
-                                                                    (Pulse_Elaborate_Pure.elab_term
-                                                                    q1)))
+                                                                    elab_p
+                                                                    elab_q))
                                                                     (fun
                                                                     uu___4 ->
                                                                     (fun
@@ -171,8 +223,38 @@ let (check_rewrite :
                                                                     match uu___4
                                                                     with
                                                                     | 
-                                                                    (FStar_Pervasives_Native.None,
+                                                                    (res,
                                                                     issues)
+                                                                    ->
+                                                                    Obj.magic
+                                                                    (FStar_Tactics_Effect.tac_bind
+                                                                    (FStar_Sealed.seal
+                                                                    (Obj.magic
+                                                                    (FStar_Range.mk_range
+                                                                    "Pulse.Checker.Rewrite.fst"
+                                                                    (Prims.of_int (30))
+                                                                    (Prims.of_int (11))
+                                                                    (Prims.of_int (30))
+                                                                    (Prims.of_int (30)))))
+                                                                    (FStar_Sealed.seal
+                                                                    (Obj.magic
+                                                                    (FStar_Range.mk_range
+                                                                    "Pulse.Checker.Rewrite.fst"
+                                                                    (Prims.of_int (31))
+                                                                    (Prims.of_int (11))
+                                                                    (Prims.of_int (40))
+                                                                    (Prims.of_int (30)))))
+                                                                    (Obj.magic
+                                                                    (FStar_Tactics_V2_Builtins.log_issues
+                                                                    issues))
+                                                                    (fun
+                                                                    uu___5 ->
+                                                                    (fun
+                                                                    uu___5 ->
+                                                                    match res
+                                                                    with
+                                                                    | 
+                                                                    FStar_Pervasives_Native.None
                                                                     ->
                                                                     Obj.magic
                                                                     (Obj.repr
@@ -181,69 +263,241 @@ let (check_rewrite :
                                                                     (Obj.magic
                                                                     (FStar_Range.mk_range
                                                                     "Pulse.Checker.Rewrite.fst"
-                                                                    (Prims.of_int (29))
-                                                                    (Prims.of_int (25))
-                                                                    (Prims.of_int (30))
-                                                                    (Prims.of_int (50)))))
+                                                                    (Prims.of_int (34))
+                                                                    (Prims.of_int (20))
+                                                                    (Prims.of_int (38))
+                                                                    (Prims.of_int (53)))))
                                                                     (FStar_Sealed.seal
                                                                     (Obj.magic
                                                                     (FStar_Range.mk_range
                                                                     "Pulse.Checker.Rewrite.fst"
-                                                                    (Prims.of_int (29))
+                                                                    (Prims.of_int (33))
                                                                     (Prims.of_int (13))
-                                                                    (Prims.of_int (30))
-                                                                    (Prims.of_int (50)))))
+                                                                    (Prims.of_int (38))
+                                                                    (Prims.of_int (53)))))
                                                                     (Obj.magic
                                                                     (FStar_Tactics_Effect.tac_bind
                                                                     (FStar_Sealed.seal
                                                                     (Obj.magic
                                                                     (FStar_Range.mk_range
                                                                     "Pulse.Checker.Rewrite.fst"
-                                                                    (Prims.of_int (30))
-                                                                    (Prims.of_int (26))
-                                                                    (Prims.of_int (30))
-                                                                    (Prims.of_int (49)))))
+                                                                    (Prims.of_int (38))
+                                                                    (Prims.of_int (27))
+                                                                    (Prims.of_int (38))
+                                                                    (Prims.of_int (52)))))
                                                                     (FStar_Sealed.seal
                                                                     (Obj.magic
                                                                     (FStar_Range.mk_range
-                                                                    "prims.fst"
-                                                                    (Prims.of_int (590))
-                                                                    (Prims.of_int (19))
-                                                                    (Prims.of_int (590))
-                                                                    (Prims.of_int (31)))))
+                                                                    "Pulse.Checker.Rewrite.fst"
+                                                                    (Prims.of_int (34))
+                                                                    (Prims.of_int (20))
+                                                                    (Prims.of_int (38))
+                                                                    (Prims.of_int (53)))))
                                                                     (Obj.magic
-                                                                    (Pulse_Typing_Env.print_issues
-                                                                    g1 issues))
-                                                                    (fun
-                                                                    uu___5 ->
-                                                                    FStar_Tactics_Effect.lift_div_tac
+                                                                    (FStar_Tactics_V2_Builtins.term_to_string
+                                                                    elab_q))
                                                                     (fun
                                                                     uu___6 ->
+                                                                    (fun
+                                                                    uu___6 ->
+                                                                    Obj.magic
+                                                                    (FStar_Tactics_Effect.tac_bind
+                                                                    (FStar_Sealed.seal
+                                                                    (Obj.magic
+                                                                    (FStar_Range.mk_range
+                                                                    "Pulse.Checker.Rewrite.fst"
+                                                                    (Prims.of_int (34))
+                                                                    (Prims.of_int (20))
+                                                                    (Prims.of_int (38))
+                                                                    (Prims.of_int (53)))))
+                                                                    (FStar_Sealed.seal
+                                                                    (Obj.magic
+                                                                    (FStar_Range.mk_range
+                                                                    "Pulse.Checker.Rewrite.fst"
+                                                                    (Prims.of_int (34))
+                                                                    (Prims.of_int (20))
+                                                                    (Prims.of_int (38))
+                                                                    (Prims.of_int (53)))))
+                                                                    (Obj.magic
+                                                                    (FStar_Tactics_Effect.tac_bind
+                                                                    (FStar_Sealed.seal
+                                                                    (Obj.magic
+                                                                    (FStar_Range.mk_range
+                                                                    "Pulse.Checker.Rewrite.fst"
+                                                                    (Prims.of_int (37))
+                                                                    (Prims.of_int (27))
+                                                                    (Prims.of_int (37))
+                                                                    (Prims.of_int (52)))))
+                                                                    (FStar_Sealed.seal
+                                                                    (Obj.magic
+                                                                    (FStar_Range.mk_range
+                                                                    "Pulse.Checker.Rewrite.fst"
+                                                                    (Prims.of_int (34))
+                                                                    (Prims.of_int (20))
+                                                                    (Prims.of_int (38))
+                                                                    (Prims.of_int (53)))))
+                                                                    (Obj.magic
+                                                                    (FStar_Tactics_V2_Builtins.term_to_string
+                                                                    elab_p))
+                                                                    (fun
+                                                                    uu___7 ->
+                                                                    (fun
+                                                                    uu___7 ->
+                                                                    Obj.magic
+                                                                    (FStar_Tactics_Effect.tac_bind
+                                                                    (FStar_Sealed.seal
+                                                                    (Obj.magic
+                                                                    (FStar_Range.mk_range
+                                                                    "Pulse.Checker.Rewrite.fst"
+                                                                    (Prims.of_int (34))
+                                                                    (Prims.of_int (20))
+                                                                    (Prims.of_int (38))
+                                                                    (Prims.of_int (53)))))
+                                                                    (FStar_Sealed.seal
+                                                                    (Obj.magic
+                                                                    (FStar_Range.mk_range
+                                                                    "Pulse.Checker.Rewrite.fst"
+                                                                    (Prims.of_int (34))
+                                                                    (Prims.of_int (20))
+                                                                    (Prims.of_int (38))
+                                                                    (Prims.of_int (53)))))
+                                                                    (Obj.magic
+                                                                    (FStar_Tactics_Effect.tac_bind
+                                                                    (FStar_Sealed.seal
+                                                                    (Obj.magic
+                                                                    (FStar_Range.mk_range
+                                                                    "Pulse.Checker.Rewrite.fst"
+                                                                    (Prims.of_int (36))
+                                                                    (Prims.of_int (27))
+                                                                    (Prims.of_int (36))
+                                                                    (Prims.of_int (47)))))
+                                                                    (FStar_Sealed.seal
+                                                                    (Obj.magic
+                                                                    (FStar_Range.mk_range
+                                                                    "Pulse.Checker.Rewrite.fst"
+                                                                    (Prims.of_int (34))
+                                                                    (Prims.of_int (20))
+                                                                    (Prims.of_int (38))
+                                                                    (Prims.of_int (53)))))
+                                                                    (Obj.magic
+                                                                    (Pulse_Syntax_Printer.term_to_string
+                                                                    q1))
+                                                                    (fun
+                                                                    uu___8 ->
+                                                                    (fun
+                                                                    uu___8 ->
+                                                                    Obj.magic
+                                                                    (FStar_Tactics_Effect.tac_bind
+                                                                    (FStar_Sealed.seal
+                                                                    (Obj.magic
+                                                                    (FStar_Range.mk_range
+                                                                    "Pulse.Checker.Rewrite.fst"
+                                                                    (Prims.of_int (34))
+                                                                    (Prims.of_int (20))
+                                                                    (Prims.of_int (38))
+                                                                    (Prims.of_int (53)))))
+                                                                    (FStar_Sealed.seal
+                                                                    (Obj.magic
+                                                                    (FStar_Range.mk_range
+                                                                    "Pulse.Checker.Rewrite.fst"
+                                                                    (Prims.of_int (34))
+                                                                    (Prims.of_int (20))
+                                                                    (Prims.of_int (38))
+                                                                    (Prims.of_int (53)))))
+                                                                    (Obj.magic
+                                                                    (FStar_Tactics_Effect.tac_bind
+                                                                    (FStar_Sealed.seal
+                                                                    (Obj.magic
+                                                                    (FStar_Range.mk_range
+                                                                    "Pulse.Checker.Rewrite.fst"
+                                                                    (Prims.of_int (35))
+                                                                    (Prims.of_int (27))
+                                                                    (Prims.of_int (35))
+                                                                    (Prims.of_int (47)))))
+                                                                    (FStar_Sealed.seal
+                                                                    (Obj.magic
+                                                                    (FStar_Range.mk_range
+                                                                    "FStar.Printf.fst"
+                                                                    (Prims.of_int (121))
+                                                                    (Prims.of_int (8))
+                                                                    (Prims.of_int (123))
+                                                                    (Prims.of_int (44)))))
+                                                                    (Obj.magic
+                                                                    (Pulse_Syntax_Printer.term_to_string
+                                                                    p1))
+                                                                    (fun
+                                                                    uu___9 ->
+                                                                    FStar_Tactics_Effect.lift_div_tac
+                                                                    (fun
+                                                                    uu___10
+                                                                    ->
+                                                                    fun x ->
+                                                                    fun x1 ->
+                                                                    fun x2 ->
                                                                     Prims.strcat
-                                                                    "rewrite: p and q elabs are not equiv\n"
                                                                     (Prims.strcat
-                                                                    uu___5 "")))))
+                                                                    (Prims.strcat
+                                                                    (Prims.strcat
+                                                                    "rewrite: could not prove equality of "
+                                                                    (Prims.strcat
+                                                                    uu___9
+                                                                    " and "))
+                                                                    (Prims.strcat
+                                                                    x
+                                                                    "\nElaborations: "))
+                                                                    (Prims.strcat
+                                                                    x1
+                                                                    " and "))
+                                                                    (Prims.strcat
+                                                                    x2 "\n")))))
                                                                     (fun
-                                                                    uu___5 ->
+                                                                    uu___9 ->
+                                                                    FStar_Tactics_Effect.lift_div_tac
                                                                     (fun
-                                                                    uu___5 ->
+                                                                    uu___10
+                                                                    ->
+                                                                    uu___9
+                                                                    uu___8))))
+                                                                    uu___8)))
+                                                                    (fun
+                                                                    uu___8 ->
+                                                                    FStar_Tactics_Effect.lift_div_tac
+                                                                    (fun
+                                                                    uu___9 ->
+                                                                    uu___8
+                                                                    uu___7))))
+                                                                    uu___7)))
+                                                                    (fun
+                                                                    uu___7 ->
+                                                                    FStar_Tactics_Effect.lift_div_tac
+                                                                    (fun
+                                                                    uu___8 ->
+                                                                    uu___7
+                                                                    uu___6))))
+                                                                    uu___6)))
+                                                                    (fun
+                                                                    uu___6 ->
+                                                                    (fun
+                                                                    uu___6 ->
                                                                     Obj.magic
                                                                     (Pulse_Typing_Env.fail
                                                                     g1
-                                                                    FStar_Pervasives_Native.None
-                                                                    uu___5))
-                                                                    uu___5)))
-                                                                    | 
                                                                     (FStar_Pervasives_Native.Some
-                                                                    token,
-                                                                    uu___5)
-                                                                    ->
+                                                                    (t.Pulse_Syntax_Base.range2))
+                                                                    uu___6))
+                                                                    uu___6)))
+                                                                    | 
+                                                                    FStar_Pervasives_Native.Some
+                                                                    token ->
                                                                     Obj.magic
                                                                     (Obj.repr
                                                                     (FStar_Tactics_Effect.lift_div_tac
                                                                     (fun
                                                                     uu___6 ->
                                                                     ()))))
+                                                                    uu___5)))
+                                                                    uu___4)))
+                                                                    uu___4)))
                                                                     uu___4))))
                                                                     (fun
                                                                     uu___3 ->
@@ -256,17 +510,17 @@ let (check_rewrite :
                                                                     (Obj.magic
                                                                     (FStar_Range.mk_range
                                                                     "Pulse.Checker.Rewrite.fst"
-                                                                    (Prims.of_int (32))
+                                                                    (Prims.of_int (41))
                                                                     (Prims.of_int (14))
-                                                                    (Prims.of_int (32))
+                                                                    (Prims.of_int (41))
                                                                     (Prims.of_int (48)))))
                                                                     (FStar_Sealed.seal
                                                                     (Obj.magic
                                                                     (FStar_Range.mk_range
                                                                     "Pulse.Checker.Rewrite.fst"
-                                                                    (Prims.of_int (33))
+                                                                    (Prims.of_int (42))
                                                                     (Prims.of_int (6))
-                                                                    (Prims.of_int (33))
+                                                                    (Prims.of_int (42))
                                                                     (Prims.of_int (72)))))
                                                                     (FStar_Tactics_Effect.lift_div_tac
                                                                     (fun
@@ -284,17 +538,17 @@ let (check_rewrite :
                                                                     (Obj.magic
                                                                     (FStar_Range.mk_range
                                                                     "Pulse.Checker.Rewrite.fst"
-                                                                    (Prims.of_int (33))
+                                                                    (Prims.of_int (42))
                                                                     (Prims.of_int (13))
-                                                                    (Prims.of_int (33))
+                                                                    (Prims.of_int (42))
                                                                     (Prims.of_int (62)))))
                                                                     (FStar_Sealed.seal
                                                                     (Obj.magic
                                                                     (FStar_Range.mk_range
                                                                     "Pulse.Checker.Rewrite.fst"
-                                                                    (Prims.of_int (33))
+                                                                    (Prims.of_int (42))
                                                                     (Prims.of_int (6))
-                                                                    (Prims.of_int (33))
+                                                                    (Prims.of_int (42))
                                                                     (Prims.of_int (72)))))
                                                                     (Obj.magic
                                                                     (Pulse_Checker_Common.try_frame_pre
